Attempt to interpret fixed translation locale
Use previous to interpret the Morello_Fixed_Address_Translation
locale, making sure all the various assumptions about (previously
stubbed) helper functions are correct. Requires new configuration
parameters, and some fighting with word/nat arithmetic, how
exciting.

The remaining unsolved problem is that the existing locale contains
duplicate fact names, including "no_cap_load_translation_events" at
least, so actually interpreting it fails. Leaving that as a TODO.

CHERI_Instantiation.thy
@@ -1394,6 +1394,7 @@ definition bounds_address :: "AccType \<Rightarrow> nat \<Rightarrow> nat" where
 
 definition valid_address :: "AccType \<Rightarrow> nat \<Rightarrow> bool" where
   "valid_address acctype addr \<equiv>
+     (addr < 2 ^ 64) \<and>
      (if s1_enabled acctype \<and> has_ttbr1 acctype \<and> bin_nth (int addr) 55
       then (if tbi_enabled acctype addr
             then addr mod 2 ^ 56 \<ge> 15 * 2 ^ 52 \<comment> \<open>addr[55..52] = 0xF\<close>
