VM_No_Translation.thy
@@ -26,16 +26,22 @@ FIXME: this just disallows HCR_EL2.E2H. To permit that
 the two reads of HCR_EL2 in ELIsInHost read the same thing.
 \<close>
 
+record no_translation_conf =
+  top_bits_pos :: bool
+  top_bits_neg :: bool
+
 fun(sequential)
-  sctlr_no_translation :: "register_value event \<Rightarrow> bool"
+  sctlr_no_translation :: "no_translation_conf \<Rightarrow> register_value event \<Rightarrow> bool"
 where
-    "sctlr_no_translation (E_read_reg nm rv) = (
+    "sctlr_no_translation conf (E_read_reg nm rv) = (
         (nm = name PSTATE_ref \<longrightarrow> ProcState_EL (the (of_regval PSTATE_ref rv)) = EL0) \<and>
         (nm = name SCTLR_EL1_ref \<longrightarrow> \<not> lsb (the (of_regval SCTLR_EL1_ref rv))) \<and>
         (nm = name HCR_EL2_ref \<longrightarrow> (let reg = (the (of_regval HCR_EL2_ref rv))
-            in \<not> (test_bit reg 34) \<and> \<not> (test_bit reg 12) \<and> \<not> (test_bit reg 0)))
+            in \<not> (test_bit reg 34) \<and> \<not> (test_bit reg 12) \<and> \<not> (test_bit reg 0))) \<and>
+        (nm = name TCR_EL1_ref \<longrightarrow> (let reg = (the (of_regval TCR_EL1_ref rv))
+            in (test_bit reg 38 = top_bits_neg conf) \<and> \<not> (test_bit reg 37 = top_bits_pos conf)))
     )"
-  | "sctlr_no_translation ev = True"
+  | "sctlr_no_translation _ ev = True"
 
 text \<open>
 Yet another Hoare logic, this one for the pure monad rather than
@@ -129,7 +135,7 @@ lemma read_reg_hoare_pure1:
 lemmas read_reg_hoare_pure = read_reg_hoare_pure1[THEN hoare_pure_meta]
 
 lemma read_PSTATE_no_translation:
-  "hoare_pure sctlr_no_translation
+  "hoare_pure (sctlr_no_translation conf)
     ((\<forall>regv. tr (E_read_reg (name PSTATE_ref) regv)) \<and> (\<forall>ps. ProcState_EL ps = EL0 \<longrightarrow> Q ps))
     (read_reg PSTATE_ref) Q E tr"
   apply (rule hoare_pure_weaken, rule read_reg_hoare_pure)
@@ -137,7 +143,7 @@ lemma read_PSTATE_no_translation:
   done
 
 lemma read_SCTLR_no_translation:
-  "hoare_pure sctlr_no_translation
+  "hoare_pure (sctlr_no_translation conf)
     ((\<forall>regv. tr (E_read_reg (name SCTLR_EL1_ref) regv)) \<and> (\<forall>sreg. \<not> lsb sreg \<longrightarrow> Q sreg))
     (read_reg SCTLR_EL1_ref) Q E tr"
   apply (rule hoare_pure_weaken, rule read_reg_hoare_pure)
@@ -184,7 +190,7 @@ abbreviation(input)
   "nmem_event \<equiv> (\<lambda>ev. \<not> (is_mem_event ev))"
 
 lemma ELIsInHost_no_translation:
-  "hoare_pure sctlr_no_translation True
+  "hoare_pure (sctlr_no_translation conf) True
     (ELIsInHost el) (\<lambda>rv. el = EL0 \<longrightarrow> rv = False) E nmem_event"
   apply (simp only: ELIsInHost_def)
   apply (simp only: and_boolM_def or_boolM_def)
@@ -201,7 +207,7 @@ lemma ELIsInHost_no_translation:
   done
 
 lemma S1TranslationRegime__1_no_translation:
-  "hoare_pure sctlr_no_translation True
+  "hoare_pure (sctlr_no_translation conf) True
     (S1TranslationRegime__1 ()) (\<lambda>el. el = EL1) E nmem_event"
   apply (simp add: S1TranslationRegime__1_def S1TranslationRegime_def)
   apply (rule hoare_pure_weaken)
@@ -213,7 +219,7 @@ lemma S1TranslationRegime__1_no_translation:
   done
 
 lemma SCTLR_read__1_no_translation:
-  "hoare_pure sctlr_no_translation True
+  "hoare_pure (sctlr_no_translation conf) True
     (SCTLR_read__1 ()) (\<lambda>sreg. \<not> lsb sreg) E nmem_event"
   apply (simp add: SCTLR_read__1_def SCTLR_read_def)
   apply (rule hoare_pure_weaken)
@@ -231,7 +237,7 @@ lemma SCTLR_read__1_no_translation:
   done
 
 lemma AArch64_IsStageOneEnabled_no_translation:
-  "hoare_pure sctlr_no_translation True
+  "hoare_pure (sctlr_no_translation conf) True
     (AArch64_IsStageOneEnabled acc_type)
     (\<lambda>x. \<not> x) E nmem_event"
   apply (simp add: AArch64_IsStageOneEnabled_def)
@@ -264,7 +270,7 @@ lemma hoare_pure_pre_cont:
   by (clarsimp simp add: hoare_pure_def)
 
 lemma AArch64_AddressSizeFault_no_translation:
-  "hoare_pure sctlr_no_translation True
+  "hoare_pure (sctlr_no_translation conf) True
     (AArch64_AddressSizeFault addr lvl acctype iswrite snd_stage s2fs)
     (\<lambda>desc. FaultRecord_statuscode desc \<noteq> Fault_None) E nmem_event"
   apply (simp add: AArch64_AddressSizeFault_def AArch64_CreateFaultRecord_def)
@@ -277,7 +283,7 @@ lemma AArch64_AddressSizeFault_no_translation:
   done
 
 lemma AArch64_AlignmentFault_no_translation:
-  "hoare_pure sctlr_no_translation True
+  "hoare_pure (sctlr_no_translation conf) True
     (AArch64_AlignmentFault acctype iswrite snd_stage)
     (\<lambda>desc. FaultRecord_statuscode desc \<noteq> Fault_None) E nmem_event"
   apply (simp add: AArch64_AlignmentFault_def AArch64_CreateFaultRecord_def)
@@ -290,7 +296,7 @@ lemma AArch64_AlignmentFault_no_translation:
   done
 
 lemma AArch64_NoFault_no_translation:
-  "hoare_pure sctlr_no_translation True
+  "hoare_pure (sctlr_no_translation conf) True
     (AArch64_NoFault uu)
     (\<lambda>desc. FaultRecord_statuscode desc = Fault_None) E nmem_event"
   apply (simp add: AArch64_NoFault_def AArch64_CreateFaultRecord_def)
@@ -309,25 +315,98 @@ lemma PAMax_simp:
 setup \<open>Monad_Trace_Subset_Exploration.install_recs
   ["Morello", "Morello_types"]
   @{thms MemAttrDefaults_def IsSecure_def
-    undefined_MemAttrHints_def AddrTop_def undefined_TLBRecord_def
-    ELUsingAArch32_def undefined_AccessDescriptor_def
+    undefined_MemAttrHints_def undefined_TLBRecord_def
+    undefined_AccessDescriptor_def
     AArch64_CheckPermission_def
 }\<close>
 setup \<open>Monad_No_Exception_Exploration.install_recs
   ["Morello", "Morello_types"]
   @{thms MemAttrDefaults_def IsSecure_def
-    undefined_MemAttrHints_def AddrTop_def undefined_TLBRecord_def
-    ELUsingAArch32_def undefined_AccessDescriptor_def
+    undefined_MemAttrHints_def undefined_TLBRecord_def
+    undefined_AccessDescriptor_def
     AArch64_CheckPermission_def
 }\<close>
 
+lemmas HaveAArch32EL_simp = HaveAArch32EL_def[simplified
+    HaveEL_simp HaveAnyAArch32_def bind_return simp_thms if_simps]
+
+lemmas ELUsingAArch32_simp = ELUsingAArch32_def[simplified
+    ELStateUsingAArch32_def ELStateUsingAArch32K_def
+    HaveAArch32EL_simp bind_return simp_thms if_simps Let_def
+    prod.case]
+
+lemma ELUsingAArch32_no_translation:
+  "hoare_pure assms True (ELUsingAArch32 el) (\<lambda>x. \<not> x) E nmem_event"
+  apply (simp add: ELUsingAArch32_simp)
+  apply (rule hoare_pure_weaken)
+   apply (rule hoare_pure_bind allI hoare_pure_return
+        hoare_pure_triv_no_exception[where f="undefined_bool _"]
+        hoare_pure_triv_no_exception[where f="IsSecureBelowEL3 _"]
+        monad_no_exception monad_trace_subset
+  )+
+  apply (simp add: range_subset_iff)
+  done
+
+definition
+  addr_length :: "no_translation_conf \<Rightarrow> 64 word \<Rightarrow> nat"
+  where
+  "addr_length conf x = (if test_bit x 55
+    then (if ~ top_bits_neg conf then 64 else 56)
+    else (if top_bits_pos conf then 64 else 56))"
+
+lemma AddrTop_no_translation:
+  "hoare_pure (sctlr_no_translation conf) True (AddrTop addr el)
+    (\<lambda>rv. el = EL0 \<longrightarrow> rv = addr_length conf addr - 1) E nmem_event"
+  apply (simp add: AddrTop_def split del: if_split)
+  apply (simp only: HaveEL_simp bind_return)
+  apply (rule hoare_pure_weaken)
+   apply (rule hoare_pure_bind allI hoare_pure_If
+        hoare_pure_return
+        read_reg_hoare_pure
+        ELIsInHost_no_translation[THEN hoare_pure_meta]
+        ELUsingAArch32_no_translation[THEN hoare_pure_meta]
+        S1TranslationRegime__1_no_translation[THEN hoare_pure_meta]
+        hoare_pure_assert_exp
+        hoare_pure_triv_no_exception[where f="undefined_bool _"]
+        hoare_pure_triv_no_exception[where f="undefined_bitvector _"]
+        monad_no_exception monad_trace_subset
+    | simp add: IsFault_def and_boolM_def S1TranslationRegime_def
+        split del: if_split cong: if_cong
+   )+
+  apply (clarsimp simp add: range_subset_iff EL0_def EL1_def EL2_def EL3_def
+        split del: if_split cong: if_cong)
+  apply (simp add: TCR_EL1_ref_def if_bool_eq_conj Let_def
+        word_eq_iff[where 'a=1] nth_slice)
+  apply (intro allI conjI impI; clarsimp simp: addr_length_def)
+  done
+
+definition
+  valid_no_translation_address :: "no_translation_conf \<Rightarrow> 64 word \<Rightarrow> bool"
+  where
+  "valid_no_translation_address conf addr =
+    (addr AND mask (addr_length conf addr) AND (NOT (mask 48)) = 0)"
+
+lemma is_zero_valid_no_translation_address:
+  "is_zero_subrange addr (of_nat (addr_length conf addr - Suc 0)) 48 \<Longrightarrow>
+    valid_no_translation_address conf addr"
+  apply (simp add: valid_no_translation_address_def is_zero_subrange_def
+        addr_length_def)
+  apply (auto simp add: mask_def slice_mask_def sail_mask_def
+        elim: subst[where P="\<lambda>x. addr AND x = _", rotated])
+  done
+
 lemma AArch64_TranslateAddressS1Off_no_translation:
-  "hoare_pure sctlr_no_translation True
+  "hoare_pure (sctlr_no_translation conf) True
     (AArch64_TranslateAddressS1Off vaddress acctype iswrite)
-    (\<lambda>rec. \<not> IsFault (TLBRecord_addrdesc rec) \<longrightarrow>
-        FullAddress_address (AddressDescriptor_paddress (TLBRecord_addrdesc rec)) = (ucast vaddress))
+    (\<lambda>rec. (\<not> IsFault (TLBRecord_addrdesc rec) \<longrightarrow>
+            FullAddress_address (AddressDescriptor_paddress (TLBRecord_addrdesc rec)) =
+                (ucast vaddress) \<and>
+            valid_no_translation_address conf vaddress) \<and>
+        (let upd = TLBRecord_descupdate rec in
+            (\<not> DescriptorUpdate_AF upd \<and> \<not> DescriptorUpdate_AP upd \<and> \<not> DescriptorUpdate_SC upd)))
     E nmem_event"
   apply (simp add: AArch64_TranslateAddressS1Off_def)
+  apply (simp only: PAMax_simp bind_return)
   apply (rule hoare_pure_weaken)
    apply (rule hoare_pure_bind allI hoare_pure_If
         hoare_pure_pair_case hoare_pure_return
@@ -336,6 +415,7 @@ lemma AArch64_TranslateAddressS1Off_no_translation:
         AArch64_AddressSizeFault_no_translation[THEN hoare_pure_meta]
         AArch64_NoFault_no_translation[THEN hoare_pure_meta]
         SCTLR_read__1_no_translation[THEN hoare_pure_meta]
+        AddrTop_no_translation[THEN hoare_pure_meta]
         read_PSTATE_no_translation
         hoare_pure_assert_exp
         S1TranslationRegime__1_no_translation[THEN hoare_pure_meta]
@@ -343,7 +423,7 @@ lemma AArch64_TranslateAddressS1Off_no_translation:
     | simp only: Let_def simp_thms and_boolM_def if_simps PAMax_simp
     | (rule hoare_pure_triv_no_exception, rule monad_no_exception)
   )+
-  apply (clarsimp simp: range_subset_iff)
+  apply (clarsimp simp: range_subset_iff is_zero_valid_no_translation_address)
   done
 
 lemma hoare_pure_throw:
@@ -379,8 +459,8 @@ lemma hoare_pure_liftR:
   apply (clarsimp simp: hoare_pure_return hoare_pure_throw split: sum.split)
   done
 
-lemma AArch64_CheckAndUpdateDescriptor_no_translation1:
-  "hoare_pure sctlr_no_translation
+lemma AArch64_CheckAndUpdateDescriptor_no_translation:
+  "hoare_pure (sctlr_no_translation conf)
     ((\<not> DescriptorUpdate_AF result \<and> \<not> DescriptorUpdate_AP result \<and> \<not> DescriptorUpdate_SC result) \<and> True)
     (AArch64_CheckAndUpdateDescriptor result fault snd_stage vaddress acctype is_w s2 hwup iswritevalidcap)
     (\<lambda>flt. FaultRecord_statuscode flt = Fault_None \<longrightarrow> FaultRecord_statuscode fault = Fault_None)
@@ -395,24 +475,14 @@ lemma AArch64_CheckAndUpdateDescriptor_no_translation1:
         hoare_pure_triv_no_exception[where f="undefined_bitvector _"]
         hoare_pure_triv_no_exception[where f="undefined_AddressDescriptor _"]
         hoare_pure_triv_no_exception[where f="undefined_AccessDescriptor _"]
-        monad_no_exception monad_trace_subset)+
+        monad_no_exception monad_trace_subset
+    | simp only: if_simps or_boolM_def
+    | simp)+
   apply (clarsimp simp: range_subset_iff)
   done
 
-lemma AArch64_CheckAndUpdateDescriptor_no_translation:
-  "hoare_pure sctlr_no_translation
-    True
-    (AArch64_CheckAndUpdateDescriptor result fault snd_stage vaddress acctype is_w s2 hwup iswritevalidcap)
-    (\<lambda>flt. FaultRecord_statuscode flt = Fault_None \<longrightarrow> FaultRecord_statuscode fault = Fault_None)
-    E nmem_event"
-  (* cheated at this point. there is a semantic disagreement issue
-     about whether the AF/AP/SC update flags really get initialised
-     or not, so we cheat to hide those assumptions from the previous.
-  *)
-  sorry
-
 lemma AArch64_InstructionDevice_no_translation:
-  "hoare_pure sctlr_no_translation True
+  "hoare_pure (sctlr_no_translation conf) True
     (AArch64_InstructionDevice addrdesc vaddress ipaddress level acctype iswrite snd_stage s2fs)
     (\<lambda> desc. (\<not> IsFault desc \<longrightarrow> \<not> IsFault addrdesc) \<and>
         AddressDescriptor_paddress desc = AddressDescriptor_paddress addrdesc)
@@ -426,10 +496,11 @@ lemma AArch64_InstructionDevice_no_translation:
   done
 
 lemma AArch64_FirstStageTranslateWithTag_no_translation:
-  "hoare_pure sctlr_no_translation True
+  "hoare_pure (sctlr_no_translation conf) True
     (AArch64_FirstStageTranslateWithTag vaddress acctype iswrite wasaligned sz isw_v_cap)
     (\<lambda> desc. \<not> IsFault desc \<longrightarrow>
-        FullAddress_address (AddressDescriptor_paddress desc) = (ucast vaddress))
+        FullAddress_address (AddressDescriptor_paddress desc) = (ucast vaddress)
+            \<and> valid_no_translation_address conf vaddress)
     E nmem_event"
   apply (simp add: AArch64_FirstStageTranslateWithTag_def)
   apply (rule hoare_pure_weaken)
@@ -449,10 +520,11 @@ lemma AArch64_FirstStageTranslateWithTag_no_translation:
     | simp add: IsFault_def split del: if_split
   )+
   apply (clarsimp simp: IsFault_def range_subset_iff)
+  apply auto
   done
 
 lemma AArch64_SecondStageTranslate_no_translation:
-  "hoare_pure sctlr_no_translation True
+  "hoare_pure (sctlr_no_translation conf) True
     (AArch64_SecondStageTranslate S1 vaddress acctype iswrite wasaligned s2fs sz hwup isw_v_cap)
     (\<lambda> desc. desc = S1)
     E nmem_event"
@@ -478,11 +550,17 @@ lemma AArch64_SecondStageTranslate_no_translation:
         word_eq_iff[where 'a=1] nth_slice nth_ucast)
   done
 
+definition check_translate_address :: "no_translation_conf \<Rightarrow> nat \<Rightarrow> nat option" where
+  "check_translate_address conf addr =
+    (if addr < 2 ^ 64 \<and> valid_no_translation_address conf (of_nat addr)
+    then Some (addr mod 2^48) else None)"
+
 lemma AArch64_FullTranslateWithTag_no_translation:
-  "hoare_pure sctlr_no_translation True
+  "hoare_pure (sctlr_no_translation conf) True
     (AArch64_FullTranslateWithTag vaddress acctype iswrite wasaligned sz isw_v_cap)
     (\<lambda> desc. \<not> IsFault desc \<longrightarrow>
-        FullAddress_address (AddressDescriptor_paddress desc) = (ucast vaddress))
+        check_translate_address conf (unat vaddress) =
+        Some (unat (FullAddress_address (AddressDescriptor_paddress desc))))
     E nmem_event"
   apply (simp add: AArch64_FullTranslateWithTag_def)
   apply (rule hoare_pure_weaken)
@@ -496,52 +574,167 @@ lemma AArch64_FullTranslateWithTag_no_translation:
     | (rule hoare_pure_triv_no_exception, rule monad_no_exception)
   )+
   apply (clarsimp simp: range_subset_iff)
+  apply (simp add: check_translate_address_def unat_and_mask)
   done
 
-lemma translate_correct:
-  "Run (AArch64_FullTranslateWithTag vaddress acctype iswrite algnd sz is_wvc) t addrdesc \<Longrightarrow>
-    \<not>IsFault addrdesc \<Longrightarrow>
-    \<forall>e \<in> set t. sctlr_no_translation e \<Longrightarrow>
-    translate_address (unat vaddress) =
-    Some (unat (FullAddress_address (AddressDescriptor_paddress addrdesc)))"
-  apply (drule AArch64_FullTranslateWithTag_no_translation[THEN hoare_pure_RunD], simp_all)
-  apply (simp add: CHERI_Instantiation.translate_address_def unat_and_mask)
+lemma addr_length_bounds_calculation:
+  "Morello_Bounds_Address_Calculation (\<lambda>_ addr. \<not> addr_length conf (of_nat addr) = 64)"
+  apply unfold_locales
+  apply (simp add: addr_length_def test_bit_nat)
+  done
+
+lemma and_not_mask_0_imp_lt:
+  "x AND NOT (mask n) = 0 \<Longrightarrow> n < size x \<Longrightarrow> x < 2 ^ n"
+  apply (drule and_mask_less_size)
+  apply (simp only: word_minus_word_and_not_mask[symmetric])
+  apply simp
+  done
+
+lemma valid_no_translation_address_unat_lt:
+  "valid_no_translation_address conf addr \<Longrightarrow>
+    unat addr mod (2 ^ addr_length conf addr) < 2 ^ 48"
+  apply (simp add: valid_no_translation_address_def word_bw_assocs[symmetric])
+  apply (drule and_not_mask_0_imp_lt, simp)
+  apply (simp add: word_less_nat_alt unat_and_mask)
+  apply (simp add: addr_length_def split: if_split_asm)
+  done
+
+lemma check_translate_address_valid:
+  "check_translate_address conf vaddr = Some paddr \<Longrightarrow>
+    Morello_Bounds_Address_Calculation.valid_address (\<lambda>_. EL0) (\<lambda>_. False)
+        (\<lambda>_ addr. \<not> addr_length conf (of_nat addr) = 64) (\<lambda>_. False) acctype vaddr"
+  apply (simp add: addr_length_bounds_calculation
+        Morello_Bounds_Address_Calculation.valid_address_def
+        check_translate_address_def
+    split: if_split_asm)
+  apply (frule valid_no_translation_address_unat_lt)
+  apply (simp add: unat_of_nat)
+  apply (simp add: addr_length_def split: if_split_asm)
+  done
+
+lemma AArch64_AccessUsesEL_no_translation:
+  "hoare_pure (sctlr_no_translation conf) True (AArch64_AccessUsesEL acctype)
+    ((=) EL0) E nmem_event"
+  apply (simp add: AArch64_AccessUsesEL_def split del: if_split)
+  apply (rule hoare_pure_weaken)
+   apply (rule hoare_pure_return hoare_pure_If hoare_pure_bind allI read_PSTATE_no_translation)+
+  apply simp
   done
 
 lemma mod_div_cong:
   "(x :: ('a :: semiring_modulo)) mod d = y mod d \<Longrightarrow> x div d = y div d \<Longrightarrow> x = y"
   by (metis mod_mult_div_eq)
 
-interpretation fixed_no_translate:
+lemma of_nat_mod_mask:
+  "of_nat (x mod (2 ^ m)) = of_nat x AND mask m"
+  apply (rule word_unat.Rep_eqD, simp add: unat_of_nat)
+  apply (simp add: unat_and_mask unat_of_nat)
+  apply (simp add: Parity.mod_exp_eq)
+  apply (simp add: min.absorb2)
+  done
+
+lemma check_translate_address_mod_56:
+  "Morello_Bounds_Address_Calculation.valid_address (\<lambda>_. EL0) (\<lambda>_. False)
+        (\<lambda>_ addr. \<not> addr_length conf (of_nat addr) = 64) (\<lambda>_. False) acctype vaddr \<Longrightarrow>
+    check_translate_address conf (vaddr mod 2 ^ 56) =
+    check_translate_address conf vaddr"
+  using less_mask_eq[of "of_nat vaddr :: 64 word" 56, simplified word_less_nat_alt]
+  apply (simp add: check_translate_address_def mod_mod_cancel
+                   Morello_Bounds_Address_Calculation.valid_address_def
+                   addr_length_bounds_calculation)
+  apply (simp add: valid_no_translation_address_def of_nat_mod_mask[where m=56, simplified])
+  apply (simp add: addr_length_def word_ops_nth_size word_bw_assocs)
+  apply (simp split: if_split_asm add: unat_of_nat word_bw_assocs[symmetric])
+  done
+
+lemma addr_length_mask_out:
+  "n < 55 \<Longrightarrow> addr_length conf (vaddr AND NOT (mask n)) = addr_length conf vaddr"
+  by (simp add: addr_length_def word_ops_nth_size)
+
+lemma valid_no_translation_address_mask_out:
+  "n < 48 \<Longrightarrow>
+    valid_no_translation_address conf (vaddr AND NOT (mask n)) =
+    valid_no_translation_address conf vaddr"
+  apply (simp add: valid_no_translation_address_def)
+  apply (rule arg_cong2[where f="(=)"], simp_all)
+  apply (simp add: addr_length_mask_out)
+  apply (auto simp add: word_eq_iff word_ops_nth_size)
+  done
+
+lemma word_plus_is_or:
+  fixes x :: "('a :: len0) word"
+  shows "x AND y = 0 \<Longrightarrow> x + y = x OR y"
+  using word_plus_and_or[of x y]
+  by simp
+
+lemma check_translate_address_page:
+  "check_translate_address conf vaddr = map_option
+    (\<lambda>x. x + (vaddr mod (2 ^ 12)))
+    (id check_translate_address conf (vaddr - (vaddr mod (2 ^ 12))))"
+  apply (simp add: check_translate_address_def)
+  apply (simp add: of_nat_diff of_nat_mod_mask[where m=12, simplified])
+  apply (simp add: valid_no_translation_address_mask_out)
+  apply (simp add: td_gal_lt[where b="2 ^ 52" and c="2 ^ 12", simplified])
+  apply (simp add: minus_mod_eq_mult_div)
+  apply clarsimp
+  apply (simp add: minus_mod_eq_mult_div[symmetric])
+  apply (rule word_unat.Abs_eqD[where 'a=64], simp_all add: unats_def)
+  apply (simp add: of_nat_mod_mask[where m=48, simplified]
+       of_nat_mod_mask[where m=12, simplified] of_nat_diff)
+  apply (subst word_plus_is_or)
+   apply (rule word_eqI, simp add: word_ops_nth_size)
+  apply (rule word_eqI, simp add: word_ops_nth_size)
+  apply auto
+  done
+
+lemma check_translate_address_page_aligned:
+  "check_translate_address conf vaddr = Some paddr \<Longrightarrow>
+    (paddr mod 2 ^ 12) = (vaddr mod 2 ^ 12)"
+  apply (simp add: check_translate_address_def split: if_split_asm)
+  apply (clarsimp simp: mod_mod_cancel)
+  done
+
+lemma can_interpret_fixed_translation:
+  "Morello_Fixed_Address_Translation (\<lambda>_. EL0) (\<lambda>_. False)
+        (\<lambda>_ addr. \<not> addr_length conf (of_nat addr) = 64) (\<lambda>_. False)
+        (check_translate_address conf)
+        (\<lambda>_. False) (sctlr_no_translation conf) "
+  apply (unfold_locales; simp?;
+    (drule
+        AArch64_FullTranslateWithTag_no_translation[THEN hoare_pureD]
+        AArch64_AccessUsesEL_no_translation[THEN hoare_pureD]
+        AArch64_IsStageOneEnabled_no_translation[THEN hoare_pure_RunD]
+        AddrTop_no_translation[THEN hoare_pure_RunD]
+        ELIsInHost_no_translation[THEN hoare_pure_RunD],
+    simp+)?)
+      apply (simp add: addr_length_def test_bit_nat)
+     apply (simp add: addr_length_def)
+    apply (simp add: check_translate_address_valid)
+   apply (clarsimp simp: addr_length_bounds_calculation
+        Morello_Bounds_Address_Calculation.bounds_address_def
+        check_translate_address_mod_56[simplified])
+  apply (simp only: check_translate_address_page)
+  apply (clarsimp simp: minus_mod_eq_mult_div)
+  apply (frule check_translate_address_page_aligned)
+  apply (simp add: div_plus_div_distrib_dvd_left[simplified dvd_eq_mod_eq_0])
+  apply (simp add: minus_mod_eq_mult_div[symmetric])
+  done
+
+interpretation 
   Morello_Fixed_Address_Translation
-  where translate_address = CHERI_Instantiation.translate_address
+  where translate_address = "check_translate_address conf"
     and is_translation_event = "\<lambda>_. False"
-    and translation_assms = "sctlr_no_translation"
+    and translation_assms = "sctlr_no_translation conf"
     and s1_enabled = "\<lambda>_. False"
-  apply unfold_locales
-defer (* what is tbi_enabled ? *)
-  apply (simp add: translate_correct)
-apply (drule AArch64_FullTranslateWithTag_no_translation[THEN hoare_pureD], simp_all)[1]
-  apply simp
-defer (* what is translation_el ? *)
-  apply (drule AArch64_IsStageOneEnabled_no_translation[THEN hoare_pure_RunD], simp_all)[1]
-defer (* more tbi_enabled *)
-defer (* in_host *)
-apply (subst Morello_Bounds_Address_Calculation.valid_address_def)
-defer (* more tbi_enabled *)
-apply (simp add: CHERI_Instantiation.translate_address_def)
-(* I don't think this is true ... translation doesn't fail just because
-   you're out of bounds, does it? *)
-defer
-apply (subst Morello_Bounds_Address_Calculation.bounds_address_def)
-defer (* more tbi_enabled *)
-apply (simp add: CHERI_Instantiation.translate_address_def mod_mod_cancel)
-apply (simp add: CHERI_Instantiation.translate_address_def)
-apply clarsimp
-apply (rule mod_div_cong[where d="2 ^ 12"]; simp)
-apply (simp add: mod_mod_cancel)
-apply (simp add: div_exp_mod_exp_eq[where n=12 and m=36, simplified, symmetric])
-(* that's all we can do without figuring out tbi_enabled *)
-oops
+    and in_host = "\<lambda>_. False"
+    and translation_el = "\<lambda>_. EL0"
+    and tbi_enabled = "\<lambda>_ addr. addr_length conf (of_nat addr) \<noteq> 64"
+    for conf
+  apply (rule can_interpret_fixed_translation)
+  (* doesn't work because interpreting the locale creates name
+     conflicts, which is generally horrible
+  done
+  *)
+  oops
 
 end
